skip_list/key_equiv.v
@@ -4,130 +4,122 @@ From Coq Require Import Sorting.Sorted.
 From iris.algebra Require Import gset.
 
 From SkipList.lib Require Import misc.
-From SkipList.skip_list Require Import node_rep.
+From SkipList.skip_list Require Import node_lt code node_rep.
 
 
 Local Open Scope Z.
 
-Definition key_equiv (S: gset node_rep) (Skeys: gset Z) :=
-  Permutation (elements Skeys) (map node_key (elements S)).
+Module KeyEquiv (Params: SKIP_LIST_PARAMS).
+  Import Params.
+  Module NodeLt := NodeLt Params.
+  Export NodeLt.
 
-Lemma key_equiv_in (rep: node_rep) (S: gset node_rep) (Skeys: gset Z):
-  key_equiv S Skeys →
-  rep ∈ S →
-  node_key rep ∈ Skeys.
-Proof.
-  intros Hperm Hin.
-  rewrite -elem_of_elements Hperm elem_of_list_In.
-  by apply in_map, elem_of_list_In, elem_of_elements.
-Qed.
 
-Lemma key_equiv_nin (rep: node_rep) (S: gset node_rep) (Skeys: gset Z):
-  key_equiv S Skeys →
-  ¬ node_key rep ∈ Skeys →
-  ¬ rep ∈ S.
-Proof.
-  intros ? Hnin Hin.
-  by eapply Hnin, key_equiv_in.
-Qed.
+  Definition key_equiv (S: gset node_rep) (Skeys: gset Z) :=
+    Permutation (elements Skeys) (map node_key (elements S)).
 
-Lemma key_equiv_insert_nin (rep: node_rep) (S: gset node_rep) (Skeys: gset Z):
-  key_equiv S Skeys →
-  ¬ (node_key rep ∈ Skeys) →
-  key_equiv (S ∪ {[ rep ]}) (Skeys ∪ {[ node_key rep ]}).
-Proof.
-  rewrite /key_equiv.
-  intros ? Hnin.
-  rewrite union_comm [a in Permutation _ (map _ (elements a))]@union_comm.
-  rewrite ?elements_union_singleton //=.
-  *** econstructor; eauto.
-  *** eapply key_equiv_nin; eauto.
-Qed.
 
-Lemma key_equiv_subseteq (S1 S2: gset node_rep) (S1_keys S2_keys: gset Z) :
-  key_equiv S1 S1_keys →
-  key_equiv S2 S2_keys →
-  S1 ⊆ S2 →
-  S1_keys ⊆ S2_keys.
-Proof.
-  intros Hequiv1 Hequiv2 Hsub x Hin.
-  rewrite /key_equiv in Hequiv1.
-  rewrite -elem_of_elements elem_of_list_In Hequiv1 in Hin.
-  apply in_map_iff in Hin. 
-  inversion Hin as [rep (? & ?)]; subst.
-  eapply key_equiv_in, Hsub; eauto.
-  by rewrite -elem_of_elements elem_of_list_In.
-Qed.
+  Lemma key_equiv_in (rep: node_rep) (S: gset node_rep) (Skeys: gset Z):
+    key_equiv S Skeys →
+    rep ∈ S →
+    node_key rep ∈ Skeys.
+  Proof.
+    intros Hperm Hin.
+    rewrite -elem_of_elements Hperm elem_of_list_In.
+    by apply in_map, elem_of_list_In, elem_of_elements.
+  Qed.
 
-Lemma key_equiv_union (S S1 S2: gset node_rep) (Skeys S1_keys S2_keys: gset Z) :
-  key_equiv S Skeys →
-  key_equiv S1 S1_keys →
-  key_equiv S2 S2_keys →
-  S1 ∪ S2 ⊆ S →
-  S1_keys ∪ S2_keys ⊆ Skeys →
-  key_equiv (S1 ∪ S2) (S1_keys ∪ S2_keys).
-Proof.
-  intros Hequiv Hequiv1 Hequiv2 HinS HinSkeys.
-  rewrite /key_equiv.
-  apply NoDup_Permutation.
-  + apply NoDup_elements.
-  + apply no_dup_inj_in_map; last apply NoDup_elements.
-    intros x y Hinx Hiny Hkey.
+  Lemma key_equiv_nin (rep: node_rep) (S: gset node_rep) (Skeys: gset Z):
+    key_equiv S Skeys →
+    ¬ node_key rep ∈ Skeys →
+    ¬ rep ∈ S.
+  Proof.
+    intros ? Hnin Hin.
+    by eapply Hnin, key_equiv_in.
+  Qed.
 
-    assert (List.NoDup (elements Skeys)) as Hnd'.
-    { apply NoDup_ListNoDup, NoDup_elements. }
-    pose proof (Permutation_NoDup Hequiv Hnd') as Hnd.
-    clear Hnd'. apply NoDup_ListNoDup in Hnd.
-    
-    rewrite -elem_of_list_In elem_of_elements in Hinx.
-    rewrite -elem_of_list_In elem_of_elements in Hiny.
-    assert (x ∈ S) as Hinx' by set_solver.
-    assert (y ∈ S) as Hiny' by set_solver.
-    rewrite -elem_of_elements elem_of_list_In in Hinx'.
-    rewrite -elem_of_elements elem_of_list_In in Hiny'.
+  Lemma key_equiv_insert_nin (rep: node_rep) (S: gset node_rep) (Skeys: gset Z):
+    key_equiv S Skeys →
+    ¬ (node_key rep ∈ Skeys) →
+    key_equiv (S ∪ {[ rep ]}) (Skeys ∪ {[ node_key rep ]}).
+  Proof.
+    rewrite /key_equiv.
+    intros ? Hnin.
+    rewrite union_comm [a in Permutation _ (map _ (elements a))]@union_comm.
+    rewrite ?elements_union_singleton //=.
+    *** econstructor; eauto.
+    *** eapply key_equiv_nin; eauto.
+  Qed.
 
-    induction (elements S) as [|h L]; inversion Hinx'; subst.
-    - clear IHL.
-      inversion Hnd as [|? ? Hnin]; subst.
-      destruct Hiny'; first auto.
-      rewrite Hkey elem_of_list_In in Hnin.
-      destruct Hnin. by apply in_map.
-    - inversion Hiny'; subst.
-      * clear IHL.
-        inversion Hnd as [|? ? Hnin]; subst.
-        rewrite -Hkey elem_of_list_In in Hnin.
-        destruct Hnin. by apply in_map.
-      * inversion Hnd; subst.
-        by apply IHL.
-  + intros k; split.
-    - intros Hin_elem%elem_of_elements.
-      apply elem_of_union in Hin_elem as [Hin|Hin].
-      * assert (k ∈ map node_key (elements S1)) as Hin_map.
-        { rewrite -Hequiv1 elem_of_elements //. }
-        rewrite elem_of_list_In in_map_iff in Hin_map.
+  Lemma key_equiv_subseteq (S1 S2: gset node_rep) (S1_keys S2_keys: gset Z) :
+    key_equiv S1 S1_keys →
+    key_equiv S2 S2_keys →
+    S1 ⊆ S2 →
+    S1_keys ⊆ S2_keys.
+  Proof.
+    intros Hequiv1 Hequiv2 Hsub x Hin.
+    rewrite /key_equiv in Hequiv1.
+    rewrite -elem_of_elements elem_of_list_In Hequiv1 in Hin.
+    apply in_map_iff in Hin. 
+    inversion Hin as [rep (? & ?)]; subst.
+    eapply key_equiv_in, Hsub; eauto.
+    by rewrite -elem_of_elements elem_of_list_In.
+  Qed.
+
+  Lemma key_equiv_union (L: list node_rep) (S S1 S2: gset node_rep) (S1_keys S2_keys: gset Z) :
+    Permutation L (elements S) →
+    Sorted node_lt L →
+    key_equiv S1 S1_keys →
+    key_equiv S2 S2_keys →
+    S1 ∪ S2 ⊆ S →
+    key_equiv (S1 ∪ S2) (S1_keys ∪ S2_keys).
+  Proof.
+    intros Hperm Hsort Hequiv1 Hequiv2 HinS.
+    rewrite /key_equiv.
+    apply NoDup_Permutation.
+    + apply NoDup_elements.
+    + apply no_dup_inj_in_map; last apply NoDup_elements.
+      intros x y Hinx Hiny Hkey.
+
+      rewrite -elem_of_list_In elem_of_elements in Hinx.
+      rewrite -elem_of_list_In elem_of_elements in Hiny.
+
+      apply (sorted_node_key_unique L); auto.
+      - rewrite Hperm -elem_of_list_In elem_of_elements.
+        set_solver.
+      - rewrite Hperm -elem_of_list_In elem_of_elements.
+        set_solver.
+    + intros k; split.
+      - intros Hin_elem%elem_of_elements.
+        apply elem_of_union in Hin_elem as [Hin|Hin].
+        * assert (k ∈ map node_key (elements S1)) as Hin_map.
+          { rewrite -Hequiv1 elem_of_elements //. }
+          rewrite elem_of_list_In in_map_iff in Hin_map.
+          inversion Hin_map as [rep (? & Hin_elem)]; subst.
+          rewrite elem_of_list_In in_map_iff.
+          exists rep; split; first done.
+          apply elem_of_list_In, elem_of_elements, elem_of_union_l.
+          rewrite -elem_of_elements elem_of_list_In //.
+        * assert (k ∈ map node_key (elements S2)) as Hin_map.
+          { rewrite -Hequiv2 elem_of_elements //. }
+          rewrite elem_of_list_In in_map_iff in Hin_map.
+          inversion Hin_map as [rep (? & Hin_elem)]; subst.
+          rewrite elem_of_list_In in_map_iff.
+          exists rep; split; first done.
+          apply elem_of_list_In, elem_of_elements, elem_of_union_r.
+          rewrite -elem_of_elements elem_of_list_In //.
+      - intros Hin_map%elem_of_list_In.
+        rewrite in_map_iff in Hin_map.
         inversion Hin_map as [rep (? & Hin_elem)]; subst.
-        rewrite elem_of_list_In in_map_iff.
-        exists rep; split; first done.
-        apply elem_of_list_In, elem_of_elements, elem_of_union_l.
-        rewrite -elem_of_elements elem_of_list_In //.
-      * assert (k ∈ map node_key (elements S2)) as Hin_map.
-        { rewrite -Hequiv2 elem_of_elements //. }
-        rewrite elem_of_list_In in_map_iff in Hin_map.
-        inversion Hin_map as [rep (? & Hin_elem)]; subst.
-        rewrite elem_of_list_In in_map_iff.
-        exists rep; split; first done.
-        apply elem_of_list_In, elem_of_elements, elem_of_union_r.
-        rewrite -elem_of_elements elem_of_list_In //.
-    - intros Hin_map%elem_of_list_In.
-      rewrite in_map_iff in Hin_map.
-      inversion Hin_map as [rep (? & Hin_elem)]; subst.
-      apply elem_of_list_In, elem_of_elements, elem_of_union in Hin_elem as [Hin|Hin].
-      * apply elem_of_elements, elem_of_union_l.
-        rewrite -elem_of_elements Hequiv1 elem_of_list_In in_map_iff.
-        exists rep; split; first done.
-        rewrite -elem_of_list_In elem_of_elements //.
-      * apply elem_of_elements, elem_of_union_r.
-        rewrite -elem_of_elements Hequiv2 elem_of_list_In in_map_iff.
-        exists rep; split; first done.
-        rewrite -elem_of_list_In elem_of_elements //.
-Qed.
+        apply elem_of_list_In, elem_of_elements, elem_of_union in Hin_elem as [Hin|Hin].
+        * apply elem_of_elements, elem_of_union_l.
+          rewrite -elem_of_elements Hequiv1 elem_of_list_In in_map_iff.
+          exists rep; split; first done.
+          rewrite -elem_of_list_In elem_of_elements //.
+        * apply elem_of_elements, elem_of_union_r.
+          rewrite -elem_of_elements Hequiv2 elem_of_list_In in_map_iff.
+          exists rep; split; first done.
+          rewrite -elem_of_list_In elem_of_elements //.
+  Qed.
+
+End KeyEquiv.
