skip_list/spec/contains.v
@@ -53,14 +53,14 @@ Module ContainsSpec (Params: SKIP_LIST_PARAMS).
         wp_pures. wp_lam. wp_pures.
         destruct (node_down pred) as [d|] eqn:Hcurr_down; wp_pures.
         - wp_bind (Load _).
-          iInv (levelN lvl) as (S Skeys L) "(>%Hperm & _ & _ & _ & Hown_frac & _ & Hlist)" "_".
+          iInv (levelN lvl) as (S L) "(>%Hperm & _ & _ & Hown_frac & Hlist)" "_".
           iMod "Hown_frac"; iDestruct (own_valid_2 with "Hown_frac Hown_frag") 
             as %<-%frac_auth_agree_L.
           
           destruct Hpred_range as [|Hin]; first by congruence.
           rewrite -elem_of_elements elem_of_list_In -Hperm in Hin.
           rewrite list_equiv_invert_L; last done.
-          iDestruct "Hlist" as (? ? ?) "(_ & _ & _ & _ & HP & _)".
+          iDestruct "Hlist" as (? ? ? ? ?) "(_ & _ & _ & _ & _ & HP & _)".
           iMod "HP" as %Hfalse; congruence.
         - iModIntro. iApply "HΦ". iSplit. 
           { 
@@ -77,15 +77,15 @@ Module ContainsSpec (Params: SKIP_LIST_PARAMS).
         wp_pures. wp_lam. wp_pures.
         destruct (node_down pred) as [d|] eqn:Hcurr_down; wp_pures.
         - wp_bind (Load _).
-          iInv (levelN lvl) as (S Skeys L) "(>%Hperm & >%Hsort & >%Hequiv' & Hown_auth & Hown_frac & Hown_tok & Hlist)" "Hclose".
+          iInv (levelN lvl) as (S L) "(>%Hperm & >%Hsort & Hown_auth & Hown_frac & Hlist)" "Hclose".
           iMod "Hown_frac"; iDestruct (own_valid_2 with "Hown_frac Hown_frag") 
             as %<-%frac_auth_agree_L.
 
           destruct Hpred_range as [Heq|Hin].
           * assert (d = l) as -> by congruence.
             wp_load.
-            iMod ("Hclose" with "[Hlist Hown_auth Hown_frac Hown_tok]") as "_".
-            { iNext; iExists S, Skeys, L; by iFrame. }
+            iMod ("Hclose" with "[Hlist Hown_auth Hown_frac]") as "_".
+            { iNext; iExists S, L; by iFrame. }
 
             iModIntro; wp_let.
             iApply ("IH" with "[$] [] [%]").
@@ -98,7 +98,7 @@ Module ContainsSpec (Params: SKIP_LIST_PARAMS).
             iExists S; by iFrame "# ∗". 
           * rewrite -elem_of_elements elem_of_list_In -Hperm in Hin.
             rewrite list_equiv_invert_L; last done.
-            iDestruct "Hlist" as (succ' l' γ) "(Hsucc'_range & Hsome' & Hpt' & Hlock & HP & Himp)".
+            iDestruct "Hlist" as (succ' ? ? l' γ) "(Hsucc'_range & _ & Hsome' & Hpt' & Hlock & HP & Himp)".
             iDestruct "HP" as (d' down') "(Hsome_down & Hpt_down & Hown_down' & Hdown'_key)".
             iMod "Hsome_down" as %Hsome_down; iMod "Hdown'_key" as %Hdown'_key.
 
@@ -110,8 +110,8 @@ Module ContainsSpec (Params: SKIP_LIST_PARAMS).
             iMod "Hpt_down"; wp_load.
             iPoseProof ("Himp" with "[Hpt' Hpt_down Hown_down']") as "Hlist".
             { iFrame; iExists d, down'; by iFrame. }
-            iMod ("Hclose" with "[Hown_auth Hown_frac Hown_tok Hlist]") as "_".
-            { iNext; iExists S, Skeys, L. by iFrame. }
+            iMod ("Hclose" with "[Hown_auth Hown_frac Hlist]") as "_".
+            { iNext; iExists S, L. by iFrame. }
 
             iModIntro; wp_let.
             iDestruct "Hsucc'_range" as %Hsucc'_range; iDestruct "Hsome'" as %Hsome'.
@@ -123,14 +123,14 @@ Module ContainsSpec (Params: SKIP_LIST_PARAMS).
             iExists l, down. iFrame "# ∗".
             iSplit; first done. iSplit; last done.
             iExists S; by iFrame "# ∗". 
-        - iInv (levelN lvl) as (S Skeys L) "(>%Hperm & _ & _ & _ & Hown_frac & _ & Hlist)" "_".
+        - iInv (levelN lvl) as (S L) "(>%Hperm & _ & _ & Hown_frac & Hlist)" "_".
           iMod "Hown_frac"; iDestruct (own_valid_2 with "Hown_frac Hown_frag") 
             as %<-%frac_auth_agree_L.
 
           destruct Hpred_range as [|Hin]; first by congruence.
           rewrite -elem_of_elements elem_of_list_In -Hperm in Hin.
           rewrite list_equiv_invert_L; last done.
-          iDestruct "Hlist" as (? ? ?) "(_ & _ & _ & _ & HP & _)".
+          iDestruct "Hlist" as (? ? ? ? ?) "(_ & _ & _ & _ & _ & HP & _)".
           iDestruct "HP" as (? ?) "(Hfalse & _)".
           iMod "Hfalse" as %Hfalse; congruence.
     Qed.
