skip_list/spec/insert.v
@@ -1,3 +1,5 @@
+From Coq Require Import Sorting.Sorted.
+
 From iris.algebra Require Import auth frac_auth gset.
 From iris.heap_lang Require Import proofmode.
 
@@ -35,11 +37,9 @@ Module AddSpec (Params: SKIP_LIST_PARAMS).
         ∗
         ∃ (l: loc) (γ: gname), ⌜ node_next pred = Some l ⌝
                                ∗
-                               is_lock γ (node_lock pred) (node_inv l (s_tok Γ) (node_key pred))
+                               is_lock γ (node_lock pred) (node_inv l)
                                ∗
                                l ↦{#1 / 2} (rep_to_node succ)
-                               ∗
-                               own (s_tok Γ) (GSet (Zlt_range (node_key pred) (node_key succ)))
                                ∗
                                locked γ
       }}}.
@@ -61,36 +61,43 @@ Module AddSpec (Params: SKIP_LIST_PARAMS).
       iNext; iIntros (v) "(Hnode & Hlocked)".
       wp_pures. wp_lam. wp_pures.
       rewrite Hsome; wp_match.
-      iDestruct "Hnode" as (rep) "(Hnode & Hown_tok_range)".
+      iDestruct "Hnode" as (rep) "Hnode".
 
       wp_bind (Load _).
-      iInv lvlN as (S Skeys L) "(>%Hperm & >%Hsort & >%Hequiv & Hown_auth & Hown_frac & Hown_tok & Hlist)" "Hclose".
+      iInv lvlN as (S L) "(>%Hperm & >%Hsort & Hown_auth & Hown_frac & Hlist)" "Hclose".
 
-      iMod "Hown_auth"; iAssert ((⌜ pred = head ∨ pred ∈ S ⌝ ∗ ⌜succ ∈ S ∨ succ = tail⌝)%I) 
-        with "[Hown_auth Hown_pred Hown_succ]" as "(%Hpred_range & %Hsucc_range)".
+      iMod "Hown_auth"; iAssert ⌜ pred = head ∨ In pred L ⌝%I
+        with "[Hown_auth Hown_pred]" as %Hpred_range.
       {
-        iSplit.
-        - iDestruct "Hown_pred" as "[Heq|Hown]"; first by iLeft.
-          iDestruct (own_valid_2 with "Hown_auth Hown") 
-            as %[Hvalid%gset_included]%auth_both_valid_discrete.
-          iPureIntro; right; set_solver.
-        - iDestruct "Hown_succ" as "[Hown|Heq]"; last by iRight.
-          iDestruct (own_valid_2 with "Hown_auth Hown") 
-            as %[Hvalid%gset_included]%auth_both_valid_discrete.
-          iPureIntro; left; set_solver.
+        iDestruct "Hown_pred" as "[Heq|Hown]"; first by iLeft.
+        iDestruct (own_valid_2 with "Hown_auth Hown") 
+          as %[Hvalid%gset_included]%auth_both_valid_discrete.
+        iPureIntro; right. 
+        rewrite -elem_of_list_In Hperm elem_of_elements.
+        set_solver.
       }
 
-      rewrite (list_equiv_invert L head pred); last first.
-      { by rewrite -elem_of_list_In Hperm elem_of_elements. }
-      iDestruct "Hlist" as (succ' l' γ') "(>%Hsucc'_in_L & >%Hsome' & Hpt & _ & Himp)".
+      iAssert ⌜ In succ L ∨ succ = tail ⌝%I
+        with "[Hown_auth Hown_succ]" as %Hsucc_range.
+      {
+        iDestruct "Hown_succ" as "[Hown|Heq]"; last by iRight.
+        iDestruct (own_valid_2 with "Hown_auth Hown") 
+          as %[Hvalid%gset_included]%auth_both_valid_discrete.
+        iPureIntro; left. 
+        rewrite -elem_of_list_In Hperm elem_of_elements.
+        set_solver.
+      }
+
+      rewrite (list_equiv_invert L head pred); last done.
+      iDestruct "Hlist" as (succ' ? ? l' γ') "(>%Hsucc'_in_L & _ & >%Hsome' & Hpt & _ & Himp)".
       assert (l = l') as <- by congruence.
 
       wp_load.
       iDestruct (mapsto_agree with "Hnode Hpt") as "%Hsucc".
       assert (rep = succ') as -> by by apply rep_to_node_inj.
-      iMod ("Hclose" with "[Hpt Himp Hown_auth Hown_frac Hown_tok]").
+      iMod ("Hclose" with "[Hpt Himp Hown_auth Hown_frac]").
       {
-        iNext. iExists S, Skeys, L.
+        iNext. iExists S, L.
         iPoseProof ("Himp" with "Hpt") as "Hlist".
         by iFrame.
       }
@@ -102,11 +109,11 @@ Module AddSpec (Params: SKIP_LIST_PARAMS).
         assert (succ = succ') as <-; last by iFrame "# ∗".
         apply (sorted_node_key_unique (L ++ [tail])).
         - apply node_rep_sorted_app in Hsort; by destruct Hsort.
-        - by rewrite in_inv_rev -elem_of_list_In Hperm elem_of_elements.
-        - by apply in_inv_rev. 
+        - by rewrite in_inv_rev.
+        - by rewrite in_inv_rev. 
         - congruence.
       + wp_lam. wp_pures.
-        wp_apply (release_spec with "[Hnode Hlocked Hown_tok_range]"); first done.
+        wp_apply (release_spec with "[Hnode Hlocked]"); first done.
         { iFrame "# ∗"; iExists succ'; iFrame. }
         iIntros. wp_pures.
         by iApply ("IH" with "HΦ").
@@ -142,36 +149,35 @@ Module AddSpec (Params: SKIP_LIST_PARAMS).
       wp_apply findLock_spec.
       { by iFrame "#". }
       iIntros (pred succ) "(%Hrange' & #Hown_pred & #Hown_succ & Hlock)".
-      iDestruct "Hlock" as (l γ) "(%Hsome & #Hlock & Hpt & Hown_tok_range & Hlocked)".
+      iDestruct "Hlock" as (l γ) "(%Hsome & #Hlock & Hpt & Hlocked)".
 
       wp_pures. wp_lam. wp_pures.
       case_bool_decide as Hcase; wp_if.
-      + wp_lam. wp_bind (Snd _).
-        iDestruct "Hown_succ" as "[Hown_succ|%Hsucc]"; last first.
+      + iDestruct "Hown_succ" as "[Hown_succ|%Hsucc]"; last first.
         { 
           subst; exfalso. inversion Hcase as [Heq]. 
           rewrite /node_key/tail//= in Heq; lia. 
         }
 
-        iInv lvlN as (S Skeys' L) "(>%Hperm & >%Hsort & >%Hequiv' & Hown_auth & Hown_frac & Hown_tok & Hlist)" "Hclose".
+        wp_lam. wp_bind (Snd _).
+        iInv lvlN as (S L) "(>%Hperm & >%Hsort & Hown_auth & Hown_frac & Hlist)" "Hclose".
         iMod "Hown_auth"; iDestruct (own_valid_2 with "Hown_auth Hown_succ") 
           as %[Hvalid%gset_included]%auth_both_valid_discrete.
         iMod "Hown_frac"; iDestruct (own_valid_2 with "Hown_frac Hown_frag") 
           as %Hsub%frac_auth_included_total%gset_included.
         iMod (own_update_2 with "Hown_frac Hown_frag") as "[Hown_frac Hown_frag]".
         { apply frac_auth_update, (gset_local_update_union _ _ {[ succ ]}). }
-        iMod "Hown_tok".
 
         wp_pures.
-        iMod ("Hclose" with "[Hlist Hown_auth Hown_frac Hown_tok]") as "_".
+        iMod ("Hclose" with "[Hlist Hown_auth Hown_frac]") as "_".
         {
-          iNext. iExists S, Skeys', L.
+          iNext. iExists S, L.
           assert (S ∪ {[ succ ]} ≡ S) as -> by set_solver.
           by iFrame.
         }
         iModIntro.
 
-        wp_apply (release_spec with "[Hlock Hpt Hown_tok_range Hlocked]"); first done.
+        wp_apply (release_spec with "[Hlock Hpt Hlocked]"); first done.
         { iFrame "# ∗"; iExists succ; iFrame. }
         iIntros "_". wp_pures.
         iModIntro. iApply "HΦ".
@@ -182,83 +188,112 @@ Module AddSpec (Params: SKIP_LIST_PARAMS).
         assert (key = node_key succ) as -> by congruence.
         assert (key_equiv {[ succ ]} {[ node_key succ ]}) as Hequiv''.
         { rewrite /key_equiv ?elements_singleton //. }
-        assert (Skeys ⊆ Skeys') as HsubSkeys.
-        { by apply (key_equiv_subseteq Sfrag S). }
-        assert ({[ node_key succ ]} ⊆ Skeys') as Hsub_succ.
-        { by apply (key_equiv_subseteq {[ succ ]} S). }
-        assert (Skeys ∪ {[ node_key succ ]} ⊆ Skeys') as Hsub_union_Skeys.
-        { by apply union_subseteq. }
+
         assert (Sfrag ∪ {[ succ ]} ⊆ S) as Hsub_union_S.
         { by apply union_subseteq. }
-        by apply (key_equiv_union S Sfrag {[ succ ]} Skeys' Skeys {[ node_key succ ]}).
+
+        apply node_rep_sorted_app in Hsort as [_ Hsort].
+        apply node_rep_sorted_app in Hsort as [Hsort _].
+
+        by apply (key_equiv_union L S Sfrag {[ succ ]} Skeys {[ node_key succ ]}).
       + wp_lam. wp_pures.
         rewrite Hsome; wp_match.
         wp_load. wp_let. wp_alloc l' as "Hpt'". wp_let.
         iDestruct "Hpt'" as "(Hpt' & Hpt'_dup)".
 
         assert (key ≠ node_key succ) as Hneq by congruence.
-        rewrite (Zlt_range_split_op (node_key pred) (node_key succ) key); last lia.
-        iDestruct "Hown_tok_range" as "((Htok_range1 & Htok_range2) & Htok_k)".
-
-        wp_apply (newlock_spec (node_inv l' (s_tok Γ) key) with "[Hpt'_dup Htok_range2]").
+        
+        wp_apply (newlock_spec (node_inv l') with "[Hpt'_dup]").
         { iExists succ; iFrame. }
         iIntros (lk) "#Hlock'". iDestruct "Hlock'" as (γ') "Hlock'".
-        wp_pures.
 
-        rewrite (fold_rep_to_node (key, Some l', None, lk)).
-        set (new := (key, Some l', None, lk)).
+        wp_bind (InjR _).
+        iInv lvlN as (S L) "(>%Hperm & >%Hsort & Hown_auth & Hown_frac & Hlist)" "Hclose".
         
-        wp_bind (Store _ _).
-        iInv lvlN as (S Skeys' L) "(>%Hperm & >%Hsort & >%Hequiv' & Hown_auth & Hown_frac & Hown_tok & Hlist)" "Hclose".
-        iMod "Hown_auth"; iMod "Hown_frac"; iMod "Hown_tok".
+        wp_inj.
+        iDestruct (own_valid_2 with "Hown_frac Hown_frag") 
+          as %HsubS%frac_auth_included_total%gset_included.
 
-        iAssert ((⌜ pred = head ∨ pred ∈ S ⌝)%I) 
+        iAssert ⌜ pred = head ∨ In pred L ⌝%I
           with "[Hown_auth Hown_pred]" as %Hpred_range.
         {
           iDestruct "Hown_pred" as "[Heq|Hown]"; first by iLeft.
           iDestruct (own_valid_2 with "Hown_auth Hown") 
             as %[Hvalid%gset_included]%auth_both_valid_discrete.
-          iPureIntro; right; set_solver.
+          iPureIntro; right. 
+          rewrite -elem_of_list_In Hperm elem_of_elements.
+          set_solver.
+        }
+
+        iAssert ⌜ key ∉ Skeys ⌝%I
+          with "[Hlist Hpt Hown_auth Hown_pred]" as %Hnin.
+        {
+          rewrite (list_equiv_invert L head pred); last done.
+          iDestruct "Hlist" as (succ'' L1 L2 l'' γ'') "(_ & %Hsplit & %Hsome'' & Hpt'' & _)".
+          assert (l = l'') as <- by congruence.
+          iDestruct (mapsto_agree with "Hpt Hpt''") as %Hsucc.
+          iPureIntro.
+          apply rep_to_node_inj in Hsucc. rewrite -Hsucc in Hsplit.
+
+          intros Hfalse.
+          rewrite -elem_of_elements Hequiv elem_of_list_In in_map_iff in Hfalse.
+          destruct Hfalse as [x [Hkey Hin]].
+          rewrite -elem_of_list_In elem_of_elements in Hin.
+          assert (x ∈ S) as HinS by set_solver; clear Hin.
+          rewrite -elem_of_elements -Hperm elem_of_list_In in HinS.
+          
+          apply (sorted_node_lt_nin L1 L2 pred succ x).
+          { rewrite -Hsplit //. }
+          { rewrite Hkey; lia. }
+          rewrite -Hsplit. apply in_or_app; right. apply in_or_app; by left.
+        }
+
+        iMod ("Hclose" with "[Hown_auth Hown_frac Hlist]") as "_".
+        { iNext; iExists S, L; by iFrame. }
+        clear Hperm Hsort Hpred_range HsubS S L.
+
+        iModIntro; wp_pures.
+        rewrite (fold_rep_to_node (key, Some l', None, lk)).
+        set (new := (key, Some l', None, lk)).
+        
+        wp_bind (Store _ _).
+        iInv lvlN as (S L) "(>%Hperm & >%Hsort & Hown_auth & Hown_frac & Hlist)" "Hclose".
+        iMod "Hown_auth"; iMod "Hown_frac".
+
+        iAssert ⌜ pred = head ∨ In pred L ⌝%I
+          with "[Hown_auth Hown_pred]" as %Hpred_range.
+        {
+          iDestruct "Hown_pred" as "[Heq|Hown]"; first by iLeft.
+          iDestruct (own_valid_2 with "Hown_auth Hown") 
+            as %[Hvalid%gset_included]%auth_both_valid_discrete.
+          iPureIntro; right. 
+          rewrite -elem_of_list_In Hperm elem_of_elements.
+          set_solver.
         }
 
         rewrite (list_equiv_insert head pred new succ L l l' γ'); first last.
-        { by rewrite -elem_of_list_In Hperm elem_of_elements. }
+        { done. }
         { auto. }
         { rewrite /node_key//=; rewrite /node_key in Hrange'; rewrite /node_key in Hneq; lia. }
         { rewrite /node_key//=; lia. }
 
+        iMod (own_update with "Hown_auth") as "[Hown_auth Hown_auth_frag]".
+        { apply auth_update_alloc, (gset_local_update_union _ _ {[ new ]}). }
+        iMod (own_update_2 with "Hown_frac Hown_frag") as "[Hown_frac Hown_frac_frag]".
+        { apply frac_auth_update, (gset_local_update_union _ _ {[ new ]}). }
+
         iDestruct ("Hlist" with "[Hpt Hpt' Hlock]") as "Hlist".
-        { iNext. unfold from_bot_list. by iFrame "# ∗". }
+        { iNext; by iFrame "# ∗". }
         iDestruct "Hlist" as (L') "(Hpt & Hsort & Hperm & Himp)".
         iMod "Hsort" as %Hsort'; iMod "Hperm" as %Hperm'; iMod "Hpt".
         wp_store.
 
-        iDestruct (own_valid_2 with "Hown_frac Hown_frag") 
-          as %HsubS%frac_auth_included_total%gset_included.
-        iDestruct (own_valid_2 with "Hown_tok Htok_k") as 
-            %Hdisj%gset_disj_valid_op.
-        iMod (own_update_2 with "Hown_frac Hown_frag") as "[Hown_frac Hown_frac_frag]".
-        { apply frac_auth_update, (gset_local_update_union _ _ {[ new ]}). }
-        iMod (own_update with "Hown_auth") as "[Hown_auth Hown_auth_frag]".
-        { apply auth_update_alloc, (gset_local_update_union _ _ {[ new ]}). }
-        
-        iCombine "Hown_tok Htok_k" as "Hown_tok". 
-        rewrite gset_disj_union; last done.
-
-        assert (Skeys ⊆ Skeys') as HsubSkeys.
-        { by apply (key_equiv_subseteq Sfrag S). }
-
         iDestruct "Hpt" as "(Hpt & Hpt_dup)".
-        iMod ("Hclose" with "[Hpt_dup Himp Hown_auth Hown_frac Hown_tok]") as "_".
+        iMod ("Hclose" with "[Hpt_dup Himp Hown_auth Hown_frac]") as "_".
         {
-          iNext. iExists _, _, L'. 
+          iNext. iExists _, L'. 
           iPoseProof ("Himp" with "Hpt_dup") as "Hlist".
-          iFrame. iPureIntro. split; last first.
-          {
-            split; first done.
-            apply key_equiv_insert_nin; auto.
-            set_solver.
-          }
+          iFrame. iPureIntro. split; last done.
 
           apply NoDup_Permutation.
           { 
@@ -283,7 +318,7 @@ Module AddSpec (Params: SKIP_LIST_PARAMS).
         }
 
         iModIntro. wp_pures. wp_lam. wp_pures.
-        wp_apply (release_spec with "[Hlock Hpt Hlocked Htok_range1]"); first done.
+        wp_apply (release_spec with "[Hlock Hpt Hlocked]"); first done.
         { iFrame "# ∗"; iExists new; iFrame. }
         iIntros "_". wp_pures. 
         iModIntro. iApply "HΦ".
@@ -291,7 +326,6 @@ Module AddSpec (Params: SKIP_LIST_PARAMS).
         iExists (Sfrag ∪ {[new]}).
         iFrame "# ∗". iPureIntro.
         apply key_equiv_insert_nin; auto.
-        set_solver.
 
         Unshelve. auto. (* Why ;-; *)
     Qed.
